Add support for by-field struct construction

src/go_lang/examples/logging.v
@@ -12,13 +12,13 @@ Local Coercion Var' (s: string) : expr := Var s.
  *)
 
 Module log.
-  Definition logS := mkStruct ["log_sz"; "disk_sz"].
+  Definition S := mkStruct ["sz"; "disk_sz"].
   Definition T: ty := intT * intT.
   Section fields.
     Context `{ext_ty:ext_types}.
-    Definition log_sz := structF! logS "log_sz".
-    Definition disk_sz := structF! logS "disk_sz".
-    Theorem log_sz_t Γ : Γ ⊢ log_sz : (T -> intT).
+    Definition sz := structF! S "sz".
+    Definition disk_sz := structF! S "disk_sz".
+    Theorem sz_t Γ : Γ ⊢ sz : (T -> intT).
     Proof.
       typecheck.
     Qed.
@@ -29,18 +29,16 @@ Module log.
   End fields.
 End log.
 
-Hint Resolve log.log_sz_t log.disk_sz_t : types.
-
-Import log.
+Hint Resolve log.sz_t log.disk_sz_t : types.
 
 Definition write_hdr: val :=
   λ: "log",
     let: "hdr" := NewSlice byteT #4096 in
-    UInt64Put (log_sz "log") "hdr";;
-    UInt64Put (disk_sz "log") (SliceSkip "hdr" #8);;
+    UInt64Put (log.sz "log") "hdr";;
+    UInt64Put (log.disk_sz "log") (SliceSkip "hdr" #8);;
     Write #0 "hdr".
 
-Theorem write_hdr_t Γ : Γ ⊢ write_hdr : (T -> unitT).
+Theorem write_hdr_t Γ : Γ ⊢ write_hdr : (log.T -> unitT).
 Proof.
   typecheck.
 Qed.
@@ -49,23 +47,23 @@ Definition init: val :=
   λ: "disk_sz",
   if: "disk_sz" < #1 then (zero_val log.T, #false)
   else
-    let: "log" := (#0, "disk_sz") in
+    let: "log" := buildStruct log.S ["sz" ::= #0; "disk_sz" ::= "disk_sz"] in
     write_hdr "log";;
     ("log", #true).
 
-Theorem init_t Γ : Γ ⊢ init : (intT -> T * boolT).
+Theorem init_t Γ : Γ ⊢ init : (intT -> log.T * boolT).
 Proof.
   typecheck.
 Qed.
 
 Definition get: val :=
   λ: "log" "i",
-  let: "sz" := log.log_sz "log" in
+  let: "sz" := log.sz "log" in
   if: "i" < "sz"
   then (Read (#1+"i"), #true)
   else (slice.nil, #false).
 
-Theorem get_t Γ : Γ ⊢ get : (T -> intT -> slice.T byteT * boolT).
+Theorem get_t Γ : Γ ⊢ get : (log.T -> intT -> slice.T byteT * boolT).
 Proof.
   typecheck.
 Qed.
@@ -87,7 +85,7 @@ Hint Resolve write_all_t : types.
 Definition append: val :=
   λ: "logp" "bks",
   let: "log" := !"logp" in
-  let: "sz" := log.log_sz "log" in
+  let: "sz" := log.sz "log" in
   if: #1 + "sz" + slice.len "bks" ≥ log.disk_sz "log" then
     #false
   else
@@ -97,7 +95,7 @@ Definition append: val :=
     "logp" <- "new_log";;
     #true.
 
-Theorem append_t Γ : Γ ⊢ append : (refT T -> slice.T (slice.T byteT) -> boolT).
+Theorem append_t Γ : Γ ⊢ append : (refT log.T -> slice.T (slice.T byteT) -> boolT).
 Proof.
   typecheck.
 Qed.
@@ -109,7 +107,7 @@ Definition reset: val :=
   "logp" <- "new_log";;
   #().
 
-Theorem reset_t Γ : Γ ⊢ reset : (refT T -> unitT).
+Theorem reset_t Γ : Γ ⊢ reset : (refT log.T -> unitT).
 Proof.
   typecheck.
 Qed.
@@ -122,7 +120,7 @@ Definition recover: val :=
      let: "log" := ("log_sz", "disk_sz") in
      "log".
 
-Theorem recover_t Γ : Γ ⊢ recover : (unitT -> T).
+Theorem recover_t Γ : Γ ⊢ recover : (unitT -> log.T).
 Proof.
   typecheck.
 Qed.
