src/go_lang/struct.v
@@ -18,7 +18,7 @@ Section go_lang.
 
 Fixpoint get_field_e (f0: string) (rev_fields: list string): expr :=
   match rev_fields with
-  | nil => LitV LitUnit
+  | [] => LitV LitUnit
   | [f] => if String.eqb f f0 then "v" else #()
   | f::fs => if String.eqb f f0 then Snd "v" else Fst (get_field_e f0 fs)
   end.
@@ -26,15 +26,53 @@ Fixpoint get_field_e (f0: string) (rev_fields: list string): expr :=
 Definition get_field (d:descriptor) f : val :=
   λ: "v", get_field_e f (rev d.(fields)).
 
+Fixpoint assocl_lookup {A} (field_vals: list (string * A)) (f0: string) : option A :=
+  match field_vals with
+  | [] => None
+  | (f, v)::fs => if String.eqb f f0 then Some v else assocl_lookup fs f0
+  end.
+
+Fixpoint build_struct_val
+         (field_vals: list (string * expr))
+         (rev_fields: list string) : option expr :=
+  match rev_fields with
+  | [] => None
+  | [f] => assocl_lookup field_vals f
+  | f::fs => match assocl_lookup field_vals f with
+           | Some v => match build_struct_val field_vals fs with
+                      | Some vs => Some (vs, v)%E
+                      | None => None
+                      end
+           | None => None
+           end
+  end.
+
+Definition buildStruct (d:descriptor) (fvs: list (string*expr)) : expr :=
+  match build_struct_val fvs (rev d.(fields)) with
+  | Some v => v
+  | None => LitV LitUnit
+  end.
+
 End go_lang.
 
+Declare Reduction get_field := cbv [get_field rev app get_field_e fields String.eqb Ascii.eqb eqb].
+
 Ltac make_structF desc fname :=
-  let f := eval compute [desc get_field rev app get_field_e fields String.eqb Ascii.eqb eqb]
-  in (get_field desc fname) in
+  let f := eval unfold desc in (get_field desc fname) in
+  let f := eval get_field in f in
       lazymatch f with
       | context[LitUnit] => fail "struct" desc "does not have field" fname
       | _ => exact f
       end.
 
+(* we don't use this, but just to document the relevant reduction *)
+Declare Reduction buildStruct :=
+  cbv [buildStruct
+       build_struct_val
+       rev app assocl_lookup
+       String.eqb Ascii.eqb eqb].
+
 Notation "'structF!' desc fname" := (ltac:(make_structF desc fname))
                                     (at level 0, desc, fname at next level, only parsing).
+
+Notation "f ::= v" := (@pair string expr f%string v%E) (at level 60) : expr_scope.
